splitting reducibility introduction rules + cleanups

theories/Validity/Introductions/Sigma.v
@@ -1,7 +1,7 @@
 From Coq Require Import ssrbool CRelationClasses.
 From LogRel Require Import Utils Syntax.All GenericTyping LogicalRelation.
 From LogRel.LogicalRelation Require Import Properties.
-From LogRel.LogicalRelation.Introductions Require Import Universe Poly.
+From LogRel.LogicalRelation.Introductions Require Import Universe Poly Sigma.
 From LogRel.Validity Require Import Validity Irrelevance Properties Universe Poly ValidityTactics.
 
 
@@ -11,26 +11,6 @@ Set Printing Primitive Projection Parameters.
 Section SigmaCongRed.
 
 Context `{GenericTypingProperties}.
-
-Lemma redΣdom {Γ F F' G G' l} : [Γ ||-<l> tSig F G ≅ tSig F' G'] -> [Γ ||-<l> F ≅ F'].
-Proof.
-  intros RΣ0; unshelve eapply (instKripke _ (normRedΣ RΣ0).(PolyRed.shpRed)).
-  escape; gtyping.
-Qed.
-
-Lemma redΣcod {Γ F F' G G' l} : [Γ ||-<l> tSig F G ≅ tSig F' G'] -> [Γ,, F ||-<l> G ≅ G'].
-Proof.
-  intros RΣ0; unshelve eapply (instKripkeFam _ (normRedΣ RΣ0).(PolyRed.posRed)).
-  escape; gtyping.
-Qed.
-
-Lemma redΣcodfst {Γ F F' G G' l} (RΣ: [Γ ||-<l> tSig F G ≅ tSig F' G']) [RA : [Γ ||-<l> F ≅ F']] [a a'] :
-  [_ ||-<l> a ≅ a' : _ | RA] -> [Γ ||-<l> G[a..] ≅ G'[a'..]].
-Proof.
-  intros Ra.
-  unshelve now eapply (instKripkeSubst (normRedΣ RΣ).(PolyRed.posRed)); eapply irrLR.
-  apply (redΣdom (LRSig' (normRedΣ RΣ))).
-Qed.
 
 Lemma validΣdom {Γ Γ' F F' G G' l}
   {VΓ : [||-v Γ ≅ Γ']}
@@ -77,19 +57,6 @@ Lemma SigValid {Γ Γ' F G F' G' l}
 Proof. constructor; intros; now eapply SigRed. Qed.
 End SigmaCongRed.
 
-(* Lemma up_single_subst {t σ u} : t[up_term_term σ][u..] = t[u .:  σ].
-Lemma up_subst_single {t σ a} : t[up_term_term σ][a..] = t[a .: σ].
-Proof. now asimpl. Qed. *)
-
-(* Lemma subst_wk_id_tail Γ P t : P[t .: @wk_id Γ >> tRel] = P[t..]. *)
-(* Lemma wk_id_shift {t a Γ} : t[a .: @wk_id Γ >> tRel] = t[a..].
-Proof. now bsimpl. Qed. *)
-
-(* Lemma eta_up_single_subst A σ : A[up_term_term (↑ >> σ)][(σ var_zero)..] = A[σ].
-Lemma split_valid_subst_wk_id {Γ G σ} :
- G[σ] = G[up_term_term (↑ >> σ)][σ var_zero .: (@wk_id Γ) >> tRel].
-Proof.  now rewrite wk_id_shift, up_subst_single, scons_eta'. Qed. *)
-
 
 Section SigTmValidity.
   Context `{GenericTypingProperties}.
@@ -128,7 +95,7 @@ Section SigTmValidity.
     (VFU : [ Γ ||-v< one > F ≅ F' : U | VΓ | UValid VΓ ])
     (VGU : [ Γ ,, F ||-v< one > G ≅ G' : U | validSnoc VΓ VF | VU ]).
 
-  Lemma SigCongRedU {Δ σ σ'} (tΔ : [ |-[ ta ] Δ]) (Vσ : [VΓ | Δ ||-v σ ≅ σ' : _ | tΔ])
+  Lemma SigRedU {Δ σ σ'} (tΔ : [ |-[ ta ] Δ]) (Vσ : [VΓ | Δ ||-v σ ≅ σ' : _ | tΔ])
     : [ Δ ||-< one > (tSig F G)[σ] ≅ (tSig F' G')[σ'] : U | validTyExt (UValid VΓ) tΔ Vσ ].
   Proof.
     set (RΣ := SigURedTm VU VFU VGU tΔ Vσ).
@@ -142,165 +109,14 @@ Section SigTmValidity.
       eapply UValid.
   Qed.
 
-  Lemma SigCongValidU : [ Γ ||-v< one > tSig F G ≅ tSig F' G' : U | VΓ | UValid VΓ ].
-  Proof. econstructor; intros Δ tΔ  σ σ' Vσσ'; eapply SigCongRedU. Qed.
+  Lemma SigValidU : [ Γ ||-v< one > tSig F G ≅ tSig F' G' : U | VΓ | UValid VΓ ].
+  Proof. econstructor; intros Δ tΔ  σ σ' Vσσ'; eapply SigRedU. Qed.
 
 End SigTmValidity.
 
 
-Section SigRedTmEqHelper.
-  Import SigRedTmEq.
-  Context `{GenericTypingProperties}.
-
-  Lemma isLRPair_isWfPair {Γ A A' B B' l p} (ΣA : [Γ ||-<l> tSig A B ≅ tSig A' B'])
-    (RΣ := (normRedΣ ΣA))
-    (Rp : isLRPair RΣ p) :
-      isWfPair Γ A B p.
-  Proof.
-    assert (wfΓ: [|- Γ]) by (escape ; gen_typing).
-    destruct Rp as [???? wtdom convtydom wtcod convtycod rfst rsnd|].
-    2: now econstructor.
-    pose proof (Ra := instKripkeTm wfΓ rfst).
-    pose proof (instKripkeSubst RΣ.(PolyRed.posRed) _ Ra).
-    epose proof (hb := rsnd _ wk_id wfΓ).
-    cbn -[wk_id] in *.
-    escape; rewrite <-eq_subst_scons,wk_id_ren_on in EscLhb.
-    now econstructor.
-  Qed.
-
-
-  Context {Γ l A A'} (RA : [Γ ||-Σ<l> A ≅ A'])
-    {t u} (Rt : SigRedTm RA t) (Ru : SigRedTm RA u).
-
-  (* Let Rout : [Γ ||-Σ<l> RA.(ParamRedTy.outTy)].
-  Proof.
-    apply normRedΣ0.
-    econstructor; [eapply redtywf_refl|..]; destruct RA; tea.
-    cbn in *; gen_typing.
-  Defined. *)
-
-  Lemma build_sigRedTmEq
-    (eqnf : [Γ |- nf Rt ≅ nf Ru : ParamRedTy.outTyL RA])
-    (wfΓ : [|- Γ])
-    (Rfst : [ instKripke wfΓ RA.(PolyRed.shpRed) | _ ||- tFst (nf Rt) ≅ tFst (nf Ru) : _ ])
-    (Rsnd : [ instKripkeSubst RA.(PolyRed.posRed) _ Rfst | _ ||- tSnd (nf Rt) ≅ tSnd (nf Ru) : _ ]) :
-    [LRSig' RA | _ ||- t ≅ u : _].
-  Proof.
-    unshelve eexists Rt Ru _; tea.
-    - intros; now unshelve now eapply irrLR; rewrite 2!wk_fst; eapply wkLR.
-    - intros; eapply irrLREq.
-      2: now unshelve now rewrite 2!wk_snd; eapply wkLR.
-      rewrite wk_fst; clear; now bsimpl.
-  Qed.
-
-  Lemma redtmwf_fst {F G f f'} :
-    [ Γ |- f :⤳*: f' : tSig F G ] ->
-    [ Γ |- tFst f :⤳*: tFst f' : F ].
-  Proof.
-    intros [] ; constructor; [| now eapply redtm_fst].
-    timeout 1 gen_typing.
-  Qed.
-
-  Lemma redtmwf_snd {F G f f'} :
-    [ Γ |- f :⤳*: f' : tSig F G ] ->
-    [ Γ |- G[(tFst f)..] ≅ G[(tFst f')..]] ->
-    [ Γ |- tSnd f :⤳*: tSnd f' : G[(tFst f)..] ].
-  Proof.
-    intros [] ? ; constructor; [| now eapply redtm_snd].
-    eapply ty_conv; [| now symmetry]; timeout 1 gen_typing.
-  Qed.
-
-
-End SigRedTmEqHelper.
-
-Section SigRedTmEqHelper.
-  Context `{GenericTypingProperties}.
-  Import SigRedTmEq.
-
-  Lemma build_sigRedTmEq' {Γ l F F' G G'}
-    (RΣ0 : [Γ ||-<l> tSig F G ≅ tSig F' G'])
-    (RΣ := normRedΣ RΣ0)
-    {t u} (Rt : SigRedTm RΣ t) (Ru : SigRedTm RΣ u)
-    (Rdom := redΣdom RΣ0)
-    (Rfst : [ Rdom | _ ||- tFst (nf Rt) ≅ tFst (nf Ru) : _ ])
-    (Rcod := instKripkeSubst RΣ.(PolyRed.posRed) _ Rfst)
-    (Rsnd : [ Rcod | _ ||- tSnd (nf Rt) ≅ tSnd (nf Ru) : _ ]) :
-    [LRSig' RΣ | _ ||- t ≅ u : _].
-  Proof.
-    unshelve eapply (build_sigRedTmEq _ Rt Ru).
-    1: escape; gtyping.
-    1,3: eapply irrLREq; tea; reflexivity.
-    pose proof (redΣcod RΣ0); escape.
-    eapply convtm_eta_sig; cbn in *; tea; destruct Rt, Ru; cbn in *.
-    all: first [now eapply isLRPair_isWfPair| gtyping].
-  Qed.
-
-End SigRedTmEqHelper.
-
 Section ProjRed.
-  Import SigRedTmEq.
   Context `{GenericTypingProperties}.
-
-  (* Lemma redSigRedTm {l Δ F G} {p p'}
-    (RΣ : [Δ ||-Σ<l> tSig F G])
-    (Rp : SigRedTm ΣA p) :
-    [Δ ||-<l> p ≅ p' : _ | LRSig' (normRedΣ0 RΣ)] ->
-    [Δ ||-<l> p ≅  : _ | LRSig' (normRedΣ0 RΣ)] ->
-
-SigRedTmEq.whnf *)
-
-  (* Lemma sigRedTmEqNf {l Δ F G p p'}
-    (RΣ : [Δ ||-Σ<l> tSig F G])
-    (Rp : [Δ ||-<l> p ≅ p' : _ | LRSig' (normRedΣ0 RΣ)]) :
-    [Δ ||-<l> p ≅ Rp.(redL).(nf) : _ | LRSig' (normRedΣ0 RΣ)].
-  Proof.
-    symmetry; eapply redTmEqFwd.
-    + eapply lrefl; irrelevance.
-    + eapply Rp.(redL).(red).
-    + eapply whnf.
-  Qed. *)
-
-
-  Lemma fstRed {l Δ F F' G G' p p'}
-    (RΣ : [Δ ||-<l> tSig F G ≅ tSig F' G'])
-    (RF : [Δ ||-<l> F ≅ F'])
-    (Rp : [Δ ||-<l> p ≅ p' : _ | LRSig' (normRedΣ RΣ)]) :
-    [Δ ||-<l> tFst p ≅ tFst p' : _ | RF].
-  Proof.
-    (* pose proof (redTmFwd' Rp) as []. *)
-    eapply redSubstTmEq; cycle 1.
-    + eapply redtm_fst, tmr_wf_red; exact (SigRedTmEq.red (SigRedTmEq.redL Rp)).
-    + eapply redtm_fst, tmr_wf_red.
-      eapply redtmwf_conv.
-      1:exact (SigRedTmEq.red (SigRedTmEq.redR Rp)).
-      now escape.
-    + unshelve eapply irrLR, instKripkeTm; cycle -1.
-      1: intros; rewrite <- 2!wk_fst; now unshelve eapply (SigRedTmEq.eqFst Rp).
-      escape; gtyping.
-  Qed.
-
-  Lemma sndRed {l Δ F F' G G'} {p p'}
-    (RΣ : [Δ ||-<l> tSig F G ≅ tSig F' G'])
-    (RΣn := LRSig' (normRedΣ RΣ))
-    (Rp : [Δ ||-<l> p ≅ p' : _ | RΣn])
-    (RGfstp : [Δ ||-<l> G[(tFst p)..] ≅ G'[(tFst p')..]]) :
-    [Δ ||-<l> tSnd p ≅ tSnd p' : _ | RGfstp].
-  Proof.
-    eapply redSubstTmEq; cycle 1.
-    + eapply redtm_snd, tmr_wf_red; exact (SigRedTmEq.red (SigRedTmEq.redL Rp)).
-    + eapply redtm_snd, tmr_wf_red, redtmwf_conv.
-      1: exact (SigRedTmEq.red (SigRedTmEq.redR Rp)).
-      now escape.
-    + assert (wfΔ : [|- Δ]) by (escape; gen_typing).
-      erewrite <-wk_id_ren_on, <-(wk_id_ren_on _ (tSnd (nf (redL _)))).
-      eapply irrLRConv, (SigRedTmEq.eqSnd Rp wk_id wfΔ).
-      erewrite eq_subst_scons; eapply kripkeLRlrefl.
-      1: intros; eapply (normRedΣ RΣ).(PolyRed.posRed); tea.
-      symmetry; rewrite wk_fst, 2!wk_id_ren_on.
-      eapply irrLREq; [now rewrite wk_id_ren_on|].
-      eapply fstRed; now pose proof (redTmFwd' Rp) as [].
-      Unshelve. 1: tea. now eapply redΣdom.
-  Qed.
 
   Context {l Γ Γ' F F' G G' } (VΓ : [||-v Γ ≅ Γ'])
     (VF : [Γ ||-v< l > F ≅ F' | VΓ ])
@@ -334,149 +150,6 @@ End ProjRed.
 
 Section PairRed.
   Context `{GenericTypingProperties}.
-
-  Lemma pairFstRed {Γ A A' B B' a a' b b' l}
-    (RA : [Γ ||-<l> A ≅ A'])
-    (RB : [Γ ,, A ||-<l> B ≅ B'])
-    (WtB' : [Γ ,, A' |- B'])
-    (RBa : [Γ ||-<l> B[a..] ≅ B'[a'..] ])
-    (Ra : [Γ ||-<l> a ≅ a' : A | RA])
-    (Rb : [Γ ||-<l> b ≅ b' : _ | RBa ]) :
-    [Γ ||-<l> tFst (tPair A B a b) ≅ tFst (tPair A' B' a' b') : _ | RA].
-  Proof.
-    escape.
-    eapply redSubstTmEq; tea.
-    1,2: eapply redtm_fst_beta; tea; now eapply ty_conv.
-  Qed.
-
-  Lemma pairFstRed' {Γ A A' B B' a a' b b' l}
-    (RA : [Γ ||-<l> A ≅ A'])
-    (RB : [Γ ,, A ||-<l> B ≅ B'])
-    (WtB' : [Γ ,, A' |- B'])
-    (RBa : [Γ ||-<l> B[a..] ≅ B'[a'..] ])
-    (Ra : [Γ ||-<l> a ≅ a' : A | RA])
-    (Rb : [Γ ||-<l> b ≅ b' : _ | RBa ]) :
-    [Γ ||-<l> tFst (tPair A B a b) ≅ tFst (tPair A' B' a' b') : _ | RA]
-    × [Γ ||-<l> tFst (tPair A B a b) ≅ a : _ | lrefl RA]
-    × [Γ ||-<l> tFst (tPair A' B' a' b') ≅ a' : _ | urefl RA ].
-  Proof.
-    escape.
-    eapply redSubstTmEq'; tea.
-    1,2: eapply redtm_fst_beta; tea; now eapply ty_conv.
-  Qed.
-
-  Lemma pairSndRed {Γ A A' B B' a a' b b' l}
-    (RA : [Γ ||-<l> A ≅ A'])
-    (RB : [Γ ,, A ||-<l> B ≅ B'])
-    (WtB' : [Γ ,, A' |- B'])
-    (RBa : [Γ ||-<l> B[a..] ≅ B'[a'..] ])
-    (RBfst : [Γ ||-<l> B[(tFst (tPair A B a b))..] ≅ B'[(tFst (tPair A' B' a' b'))..]])
-    (RBfsta : [Γ ||-<l> B[a..] ≅ B[(tFst (tPair A B a b))..]])
-    (Ra : [Γ ||-<l> a ≅ a' : A | RA])
-    (Rb : [Γ ||-<l> b ≅ b' : _ | RBa ]) :
-    [Γ ||-<l> tSnd (tPair A B a b) ≅ tSnd (tPair A' B' a' b') : _ | RBfst ].
-  Proof.
-    (* pose proof (LRTyEqRedRight _ RBBfst). *)
-    escape.
-    eapply redSubstTmEq; tea.
-    1: now eapply irrLRConv.
-    1,2: eapply redtm_snd_beta; tea; now eapply ty_conv.
-  Qed.
-
-  Import SigRedTmEq.
-
-  Lemma sigEtaRed {Γ A A' B B' l p p'}
-    (RΣ0 : [Γ ||-<l> tSig A B ≅ tSig A' B'])
-    (RΣn := normRedΣ RΣ0)
-    (RΣ := LRSig' RΣn)
-    (RA : [Γ ||-<l> A ≅ A'])
-    (RBfst : [Γ ||-<l> B[(tFst p)..] ≅ B'[(tFst p')..]])
-    (Rp : [Γ ||-<l> p : _ | RΣ])
-    (Rp' : [Γ ||-<l> p' : _ | RΣ])
-    (Rfstpp' : [Γ ||-<l> tFst p ≅ tFst p' : _ | RA])
-    (Rsndpp' : [Γ ||-<l> tSnd p ≅ tSnd p' : _ | RBfst]) :
-    [Γ ||-<l> p ≅ p' : _ | RΣ].
-  Proof.
-    pose proof (redTmFwd' Rp) as [Rpnf _ _ _ _]; pose proof (Rpnf1 := fstRed _ RA Rpnf).
-    pose proof (redTmFwd' Rp') as [Rpnf' _ _ _ _]; pose proof (Rpnf1' := fstRed _ RA Rpnf').
-    unshelve eapply (build_sigRedTmEq' _ Rp.(redL) Rp'.(redL)).
-    - transitivity (tFst p); [symmetry|transitivity (tFst p')]; now eapply irrLR.
-    - pose proof (RBB' := instKripkeSubst RΣn.(PolyRed.posRed)).
-      pose proof (RB := instKripkeSubst (kripkeLRlrefl RΣn.(PolyRed.posRed))).
-      pose proof (RB' := instKripkeSubst (kripkeLRurefl RΣn.(PolyRed.posRed))).
-      pose proof (RBpnf1 := RBB' _ _ _ Rpnf1); pose proof (sndRed _ Rpnf RBpnf1).
-      pose proof (RBpnf1' := RBB' _ _ _ Rpnf1'); pose proof (sndRed _ Rpnf' RBpnf1').
-      cbn in *; eapply irrLR.
-      eapply ((transLR _ _).(transRedTm) _ (tSnd p)).
-      1: symmetry; eapply irrLRConv; tea; exact (RB _ _ _ Rpnf1).
-      eapply ((transLR _ _).(transRedTm) _ (tSnd p')); tea.
-      eapply irrLRConv; [|tea].
-      eapply RBB', urefl; tea.
-      Unshelve.
-      3: eapply RB', urefl; tea.
-      eapply RB; now symmetry.
-  Qed.
-
-
-  Lemma mkPair_isLRPair {Γ A A' A1 B B' B1 a1 b1 l}
-    (RΣ0 : [Γ ||-<l> tSig A B ≅ tSig A' B'])
-    (RΣ := normRedΣ RΣ0)
-    (RA1 : [Γ ||-<l> A ≅ A1])
-    (RB1 : [Γ ||-<l> B[a1..] ≅ B1[a1..]])
-    (Ra1 : [Γ ||-<l> a1 : _ | RA1])
-    (Rb1 : [Γ ||-<l> b1 : _ | RB1])
-  : isLRPair RΣ (tPair A1 B1 a1 b1).
-  Proof.
-    escape.
-    unshelve eapply PairLRPair; tea; intros.
-    - now unshelve now eapply irrLR, wkLR.
-    - now unshelve now eapply irrLREq, wkLR; tea; rewrite subst_ren_subst_mixed.
-  Qed.
-
-  Definition pairSigRedTm {Γ A A' A1 B B' B1 a1 b1 l}
-    (RΣ0 : [Γ ||-<l> tSig A B ≅ tSig A' B'])
-    (RΣ1 : [Γ ||-<l> tSig A B ≅ tSig A1 B1])
-    (RΣ := normRedΣ RΣ0)
-    (Ra1 : [Γ ||-<l> a1 : _ | redΣdom RΣ0])
-    (Rb1 : [Γ ||-<l> b1 : _ | redΣcodfst RΣ0 Ra1])
-  : SigRedTm RΣ (tPair A1 B1 a1 b1).
-  Proof.
-    exists (tPair A1 B1 a1 b1); pose proof (RA := redΣdom RΣ1);
-      pose proof (RB := redΣcodfst RΣ1 (fst (irrLR _ RA _ _) Ra1)).
-    + eapply redtmwf_refl; cbn.
-      assert (wfΓ : [|- Γ]) by (escape ; gtyping).
-      assert [_ ||-<l> a1 : _ | urefl RA ] by now eapply irrLRConv.
-      pose proof (instKripkeFamConv wfΓ (normRedΣ RΣ1).(PolyRed.posRed)).
-      assert [_ ||-<l> b1 : _ | urefl RB ] by now eapply irrLRConv.
-      escape.
-      eapply ty_conv; [ eapply ty_pair; tea| now symmetry].
-    + now unshelve now eapply mkPair_isLRPair; eapply irrLR.
-  Defined.
-
-  Lemma pairCongRed {Γ A A' B B' a a' b b' l}
-    (RΣ0 : [Γ ||-<l> tSig A B ≅ tSig A' B'])
-    (RΣ := normRedΣ RΣ0)
-    (RΣ' := LRSig' RΣ)
-    (RA : [Γ ||-<l> A ≅ A'])
-    (RBa : [Γ ||-<l> B[a..] ≅ B'[a'..] ])
-    (Ra : [Γ ||-<l> a ≅ a' : A | RA])
-    (Rb : [Γ ||-<l> b ≅ b' : _ | RBa ]) :
-    [Γ ||-<l> tPair A B a b ≅ tPair A' B' a' b' : _ | RΣ'].
-  Proof.
-    assert (wfΓ : [|-Γ]) by (escape; gtyping).
-    pose proof (convtyB := redΣcod RΣ').
-    pose proof (wtB' := escape (symmetry (instKripkeFamConv wfΓ RΣ.(PolyRed.posRed)))).
-    unshelve epose proof (pairFstRed' RA convtyB wtB' RBa Ra Rb) as (ff'&fa&fa').
-    pose proof (RBconv := instKripkeSubst (kripkeLRlrefl RΣ.(PolyRed.posRed)) RA (fst (irrLR _ _ _ _) fa)).
-
-    unshelve eapply build_sigRedTmEq'.
-    + unshelve eapply pairSigRedTm; eapply lrefl; tea; now eapply irrLR.
-    + unshelve eapply pairSigRedTm; tea; eapply urefl. now eapply irrLR.
-      eapply irrLRConv; tea; eapply (instKripkeSubst (kripkeLRlrefl RΣ.(PolyRed.posRed)) RA Ra).
-    + cbn; eapply irrLR, pairFstRed; tea.
-    + unshelve now cbn; eapply irrLR; eapply pairSndRed; tea; symmetry.
-      now eapply (instKripkeSubst RΣ.(PolyRed.posRed)).
-  Qed.
 
   Lemma subst_sig {A B σ} : (tSig A B)[σ] = (tSig A[σ] B[up_term_term σ]).
   Proof. reflexivity. Qed.
