theories/AutoSubst/Extra.v
@@ -111,4 +111,6 @@ Proof. now asimpl. Qed.
 Definition elimSuccHypTy P :=
   tProd tNat (arr P P[tSucc (tRel 0)]⇑).
 
-Equations Derive NoConfusion Subterm for term.
+
+Equations Derive NoConfusion EqDec for sort.
+Equations Derive NoConfusion Subterm EqDec for term.
