theories/LogicalRelation/Introductions/Application.v
@@ -11,72 +11,6 @@ Smpl Add fold_subst_term : refold.
 Section Application.
 Context `{GenericTypingProperties}.
 
-
-(* Section AppTerm.
-  Context {Γ t u F G l l' l''}
-    (hΠ : [Γ ||-Π<l> tProd F G])
-    {RF : [Γ ||-<l'> F]}
-    (Rt : [Γ ||-<l> t : tProd F G | LRPi' (normRedΠ0 hΠ)])
-    (Ru : [Γ ||-<l'> u : F | RF])
-    (RGu : [Γ ||-<l''> G[u..]]).
-
-  Lemma app_id : [Γ ||-<l''> tApp (PiRedTmEq.nf Rt) u : G[u..] | RGu].
-  Proof.
-    assert (wfΓ := wfc_wft (escape RF)).
-    replace (PiRedTm.nf _) with (PiRedTm.nf Rt)⟨@wk_id Γ⟩ by now bsimpl.
-    irrelevance0.  2: eapply (PiRedTm.app Rt).
-    cbn; now bsimpl.
-    Unshelve. 1: eassumption.
-    cbn; irrelevance0; tea; now bsimpl.
-  Qed.
-
-  Lemma appTerm0 :
-      [Γ ||-<l''> tApp t u : G[u..] | RGu]
-      × [Γ ||-<l''> tApp t u ≅ tApp (PiRedTm.nf Rt) u : G[u..] | RGu].
-  Proof.
-    eapply redwfSubstTerm.
-    1: unshelve eapply app_id; tea.
-    escape.
-    eapply redtmwf_app.
-    1: apply Rt.
-    easy.
-  Qed.
-
-End AppTerm. *)
-
-(* Lemma appTerm {Γ t u F G l}
-  (RΠ : [Γ ||-<l> tProd F G])
-  {RF : [Γ ||-<l> F]}
-  (Rt : [Γ ||-<l> t : tProd F G | RΠ])
-  (Ru : [Γ ||-<l> u : F | RF])
-  (RGu : [Γ ||-<l> G[u..]]) :
-  [Γ ||-<l> tApp t u : G[u..]| RGu].
-Proof.
-  unshelve eapply appTerm0.
-  7:irrelevance.
-  3: exact (invLRΠ RΠ).
-  all: tea.
-  irrelevance.
-Qed.
-
-Lemma appTerm' {Γ t u F G l X}
-  (RΠ : [Γ ||-<l> tProd F G])
-  {RF : [Γ ||-<l> F]}
-  (Rt : [Γ ||-<l> t : tProd F G | RΠ])
-  (Ru : [Γ ||-<l> u : F | RF])
-  (eq : X = G[u..])
-  (RX : [Γ ||-<l> X]) :
-  [Γ ||-<l> tApp t u : X | RX].
-Proof.
-  irrelevance0; [symmetry; tea|].
-  unshelve eapply appTerm; cycle 1; tea.
-  Unshelve. now rewrite <- eq.
-Qed.  *)
-
-(* eq_subst_scons *)
-(* Lemma scons_wk_id {Γ t u} : t[u .: wk_id (Γ:=Γ) >> tRel] = t[u..].
-Proof. now bsimpl. Qed. *)
-
 Lemma codSubst {Γ u u' F F' G G' l l'}
   (RΠ : [Γ ||-<l> tProd F G ≅ tProd F' G'])
   {RF : [Γ ||-<l'> F ≅ F']}
@@ -112,25 +46,6 @@ Proof.
     2: eapply ty_conv; now escape.
     1: eapply redtm_conv; [now destruct (PiRedTmEq.red Rt')| now escape].
 Qed.
-
-(* Lemma appcongTerm' {Γ t t' u u' F F' G l l' X}
-  (RΠ : [Γ ||-<l> tProd F G])
-  {RF : [Γ ||-<l'> F]}
-  {RF' : [Γ ||-<l'> F']}
-  (RFF' : [Γ ||-<l'> F ≅ F' | RF])
-  (Rtt' : [Γ ||-<l> t ≅ t' : tProd F G | RΠ])
-  (Ru : [Γ ||-<l'> u : F | RF])
-  (Ru' : [Γ ||-<l'> u' : F' | RF'])
-  (Ruu' : [Γ ||-<l'> u ≅ u' : F | RF ])
-  (RGu : [Γ ||-<l'> X])
-   : X = G[u..] ->
-    [Γ ||-<l'> tApp t u ≅ tApp t' u' : X | RGu].
-Proof.
-  intros eq.
-  irrelevance0 ; [symmetry; apply eq|].
-  unshelve eapply appcongTerm; cycle 2; tea.
-  Unshelve. now rewrite <- eq.
-Qed. *)
 
 End Application.
 
