theories/LogicalRelation/Introductions/Sigma.v
@@ -1,0 +1,292 @@
+From LogRel Require Import Utils Syntax.All GenericTyping LogicalRelation.
+From LogRel.LogicalRelation Require Import Properties.
+From LogRel.LogicalRelation.Introductions Require Import Universe Poly.
+
+Set Universe Polymorphism.
+Set Printing Primitive Projection Parameters.
+
+Section SigmaRed.
+
+Context `{GenericTypingProperties}.
+
+Lemma redΣdom {Γ F F' G G' l} : [Γ ||-<l> tSig F G ≅ tSig F' G'] -> [Γ ||-<l> F ≅ F'].
+Proof.
+  intros RΣ0; unshelve eapply (instKripke _ (normRedΣ RΣ0).(PolyRed.shpRed)).
+  escape; gtyping.
+Qed.
+
+Lemma redΣcod {Γ F F' G G' l} : [Γ ||-<l> tSig F G ≅ tSig F' G'] -> [Γ,, F ||-<l> G ≅ G'].
+Proof.
+  intros RΣ0; unshelve eapply (instKripkeFam _ (normRedΣ RΣ0).(PolyRed.posRed)).
+  escape; gtyping.
+Qed.
+
+Lemma redΣcodfst {Γ F F' G G' l} (RΣ: [Γ ||-<l> tSig F G ≅ tSig F' G']) [RA : [Γ ||-<l> F ≅ F']] [a a'] :
+  [_ ||-<l> a ≅ a' : _ | RA] -> [Γ ||-<l> G[a..] ≅ G'[a'..]].
+Proof.
+  intros Ra.
+  unshelve now eapply (instKripkeSubst (normRedΣ RΣ).(PolyRed.posRed)); eapply irrLR.
+  apply (redΣdom (LRSig' (normRedΣ RΣ))).
+Qed.
+
+
+Import SigRedTmEq.
+
+Lemma isLRPair_isWfPair {Γ A A' B B' l p} (ΣA : [Γ ||-<l> tSig A B ≅ tSig A' B'])
+  (RΣ := (normRedΣ ΣA))
+  (Rp : isLRPair RΣ p) :
+    isWfPair Γ A B p.
+Proof.
+  assert (wfΓ: [|- Γ]) by (escape ; gen_typing).
+  destruct Rp as [???? wtdom convtydom wtcod convtycod rfst rsnd|].
+  2: now econstructor.
+  pose proof (Ra := instKripkeTm wfΓ rfst).
+  pose proof (instKripkeSubst RΣ.(PolyRed.posRed) _ Ra).
+  epose proof (hb := rsnd _ wk_id wfΓ).
+  cbn -[wk_id] in *.
+  escape; rewrite <-eq_subst_scons,wk_id_ren_on in EscLhb.
+  now econstructor.
+Qed.
+
+Section Helpers.
+Context {Γ l A A'} (RA : [Γ ||-Σ<l> A ≅ A'])
+  {t u} (Rt : SigRedTm RA t) (Ru : SigRedTm RA u).
+
+Lemma build_sigRedTmEq
+  (eqnf : [Γ |- nf Rt ≅ nf Ru : ParamRedTy.outTyL RA])
+  (wfΓ : [|- Γ])
+  (Rfst : [ instKripke wfΓ RA.(PolyRed.shpRed) | _ ||- tFst (nf Rt) ≅ tFst (nf Ru) : _ ])
+  (Rsnd : [ instKripkeSubst RA.(PolyRed.posRed) _ Rfst | _ ||- tSnd (nf Rt) ≅ tSnd (nf Ru) : _ ]) :
+  [LRSig' RA | _ ||- t ≅ u : _].
+Proof.
+  unshelve eexists Rt Ru _; tea.
+  - intros; now unshelve now eapply irrLR; rewrite 2!wk_fst; eapply wkLR.
+  - intros; eapply irrLREq.
+    2: now unshelve now rewrite 2!wk_snd; eapply wkLR.
+    rewrite wk_fst; clear; now bsimpl.
+Qed.
+
+Lemma redtmwf_fst {F G f f'} :
+  [ Γ |- f :⤳*: f' : tSig F G ] ->
+  [ Γ |- tFst f :⤳*: tFst f' : F ].
+Proof.
+  intros [] ; constructor; [| now eapply redtm_fst].
+  timeout 1 gen_typing.
+Qed.
+
+Lemma redtmwf_snd {F G f f'} :
+  [ Γ |- f :⤳*: f' : tSig F G ] ->
+  [ Γ |- G[(tFst f)..] ≅ G[(tFst f')..]] ->
+  [ Γ |- tSnd f :⤳*: tSnd f' : G[(tFst f)..] ].
+Proof.
+  intros [] ? ; constructor; [| now eapply redtm_snd].
+  eapply ty_conv; [| now symmetry]; timeout 1 gen_typing.
+Qed.
+End Helpers.
+
+
+Lemma build_sigRedTmEq' {Γ l F F' G G'}
+  (RΣ0 : [Γ ||-<l> tSig F G ≅ tSig F' G'])
+  (RΣ := normRedΣ RΣ0)
+  {t u} (Rt : SigRedTm RΣ t) (Ru : SigRedTm RΣ u)
+  (Rdom := redΣdom RΣ0)
+  (Rfst : [ Rdom | _ ||- tFst (nf Rt) ≅ tFst (nf Ru) : _ ])
+  (Rcod := instKripkeSubst RΣ.(PolyRed.posRed) _ Rfst)
+  (Rsnd : [ Rcod | _ ||- tSnd (nf Rt) ≅ tSnd (nf Ru) : _ ]) :
+  [LRSig' RΣ | _ ||- t ≅ u : _].
+Proof.
+  unshelve eapply (build_sigRedTmEq _ Rt Ru).
+  1: escape; gtyping.
+  1,3: eapply irrLREq; tea; reflexivity.
+  pose proof (redΣcod RΣ0); escape.
+  eapply convtm_eta_sig; cbn in *; tea; destruct Rt, Ru; cbn in *.
+  all: first [now eapply isLRPair_isWfPair| gtyping].
+Qed.
+
+Lemma fstRed {l Δ F F' G G' p p'}
+  (RΣ : [Δ ||-<l> tSig F G ≅ tSig F' G'])
+  (RF : [Δ ||-<l> F ≅ F'])
+  (Rp : [Δ ||-<l> p ≅ p' : _ | LRSig' (normRedΣ RΣ)]) :
+  [Δ ||-<l> tFst p ≅ tFst p' : _ | RF].
+Proof.
+  eapply redSubstTmEq; cycle 1.
+  + eapply redtm_fst, tmr_wf_red; exact (SigRedTmEq.red (SigRedTmEq.redL Rp)).
+  + eapply redtm_fst, tmr_wf_red.
+    eapply redtmwf_conv.
+    1:exact (SigRedTmEq.red (SigRedTmEq.redR Rp)).
+    now escape.
+  + unshelve eapply irrLR, instKripkeTm; cycle -1.
+    1: intros; rewrite <- 2!wk_fst; now unshelve eapply (SigRedTmEq.eqFst Rp).
+    escape; gtyping.
+Qed.
+
+Lemma sndRed {l Δ F F' G G'} {p p'}
+  (RΣ : [Δ ||-<l> tSig F G ≅ tSig F' G'])
+  (RΣn := LRSig' (normRedΣ RΣ))
+  (Rp : [Δ ||-<l> p ≅ p' : _ | RΣn])
+  (RGfstp : [Δ ||-<l> G[(tFst p)..] ≅ G'[(tFst p')..]]) :
+  [Δ ||-<l> tSnd p ≅ tSnd p' : _ | RGfstp].
+Proof.
+  eapply redSubstTmEq; cycle 1.
+  + eapply redtm_snd, tmr_wf_red; exact (SigRedTmEq.red (SigRedTmEq.redL Rp)).
+  + eapply redtm_snd, tmr_wf_red, redtmwf_conv.
+    1: exact (SigRedTmEq.red (SigRedTmEq.redR Rp)).
+    now escape.
+  + assert (wfΔ : [|- Δ]) by (escape; gen_typing).
+    erewrite <-wk_id_ren_on, <-(wk_id_ren_on _ (tSnd (nf (redL _)))).
+    eapply irrLRConv, (SigRedTmEq.eqSnd Rp wk_id wfΔ).
+    erewrite eq_subst_scons; eapply kripkeLRlrefl.
+    1: intros; eapply (normRedΣ RΣ).(PolyRed.posRed); tea.
+    symmetry; rewrite wk_fst, 2!wk_id_ren_on.
+    eapply irrLREq; [now rewrite wk_id_ren_on|].
+    eapply fstRed; now pose proof (redTmFwd' Rp) as [].
+    Unshelve. 1: tea. now eapply redΣdom.
+Qed.
+
+Lemma pairFstRed {Γ A A' B B' a a' b b' l}
+  (RA : [Γ ||-<l> A ≅ A'])
+  (RB : [Γ ,, A ||-<l> B ≅ B'])
+  (WtB' : [Γ ,, A' |- B'])
+  (RBa : [Γ ||-<l> B[a..] ≅ B'[a'..] ])
+  (Ra : [Γ ||-<l> a ≅ a' : A | RA])
+  (Rb : [Γ ||-<l> b ≅ b' : _ | RBa ]) :
+  [Γ ||-<l> tFst (tPair A B a b) ≅ tFst (tPair A' B' a' b') : _ | RA].
+Proof.
+  escape.
+  eapply redSubstTmEq; tea.
+  1,2: eapply redtm_fst_beta; tea; now eapply ty_conv.
+Qed.
+
+Lemma pairFstRed' {Γ A A' B B' a a' b b' l}
+  (RA : [Γ ||-<l> A ≅ A'])
+  (RB : [Γ ,, A ||-<l> B ≅ B'])
+  (WtB' : [Γ ,, A' |- B'])
+  (RBa : [Γ ||-<l> B[a..] ≅ B'[a'..] ])
+  (Ra : [Γ ||-<l> a ≅ a' : A | RA])
+  (Rb : [Γ ||-<l> b ≅ b' : _ | RBa ]) :
+  [Γ ||-<l> tFst (tPair A B a b) ≅ tFst (tPair A' B' a' b') : _ | RA]
+  × [Γ ||-<l> tFst (tPair A B a b) ≅ a : _ | lrefl RA]
+  × [Γ ||-<l> tFst (tPair A' B' a' b') ≅ a' : _ | urefl RA ].
+Proof.
+  escape.
+  eapply redSubstTmEq'; tea.
+  1,2: eapply redtm_fst_beta; tea; now eapply ty_conv.
+Qed.
+
+Lemma pairSndRed {Γ A A' B B' a a' b b' l}
+  (RA : [Γ ||-<l> A ≅ A'])
+  (RB : [Γ ,, A ||-<l> B ≅ B'])
+  (WtB' : [Γ ,, A' |- B'])
+  (RBa : [Γ ||-<l> B[a..] ≅ B'[a'..] ])
+  (RBfst : [Γ ||-<l> B[(tFst (tPair A B a b))..] ≅ B'[(tFst (tPair A' B' a' b'))..]])
+  (RBfsta : [Γ ||-<l> B[a..] ≅ B[(tFst (tPair A B a b))..]])
+  (Ra : [Γ ||-<l> a ≅ a' : A | RA])
+  (Rb : [Γ ||-<l> b ≅ b' : _ | RBa ]) :
+  [Γ ||-<l> tSnd (tPair A B a b) ≅ tSnd (tPair A' B' a' b') : _ | RBfst ].
+Proof.
+  escape.
+  eapply redSubstTmEq; tea.
+  1: now eapply irrLRConv.
+  1,2: eapply redtm_snd_beta; tea; now eapply ty_conv.
+Qed.
+
+
+Lemma sigEtaRed {Γ A A' B B' l p p'}
+  (RΣ0 : [Γ ||-<l> tSig A B ≅ tSig A' B'])
+  (RΣn := normRedΣ RΣ0)
+  (RΣ := LRSig' RΣn)
+  (RA : [Γ ||-<l> A ≅ A'])
+  (RBfst : [Γ ||-<l> B[(tFst p)..] ≅ B'[(tFst p')..]])
+  (Rp : [Γ ||-<l> p : _ | RΣ])
+  (Rp' : [Γ ||-<l> p' : _ | RΣ])
+  (Rfstpp' : [Γ ||-<l> tFst p ≅ tFst p' : _ | RA])
+  (Rsndpp' : [Γ ||-<l> tSnd p ≅ tSnd p' : _ | RBfst]) :
+  [Γ ||-<l> p ≅ p' : _ | RΣ].
+Proof.
+  pose proof (redTmFwd' Rp) as [Rpnf _ _ _ _]; pose proof (Rpnf1 := fstRed _ RA Rpnf).
+  pose proof (redTmFwd' Rp') as [Rpnf' _ _ _ _]; pose proof (Rpnf1' := fstRed _ RA Rpnf').
+  unshelve eapply (build_sigRedTmEq' _ Rp.(redL) Rp'.(redL)).
+  - transitivity (tFst p); [symmetry|transitivity (tFst p')]; now eapply irrLR.
+  - pose proof (RBB' := instKripkeSubst RΣn.(PolyRed.posRed)).
+    pose proof (RB := instKripkeSubst (kripkeLRlrefl RΣn.(PolyRed.posRed))).
+    pose proof (RB' := instKripkeSubst (kripkeLRurefl RΣn.(PolyRed.posRed))).
+    pose proof (RBpnf1 := RBB' _ _ _ Rpnf1); pose proof (sndRed _ Rpnf RBpnf1).
+    pose proof (RBpnf1' := RBB' _ _ _ Rpnf1'); pose proof (sndRed _ Rpnf' RBpnf1').
+    cbn in *; eapply irrLR.
+    eapply ((transLR _ _).(transRedTm) _ (tSnd p)).
+    1: symmetry; eapply irrLRConv; tea; exact (RB _ _ _ Rpnf1).
+    eapply ((transLR _ _).(transRedTm) _ (tSnd p')); tea.
+    eapply irrLRConv; [|tea].
+    eapply RBB', urefl; tea.
+    Unshelve.
+    3: eapply RB', urefl; tea.
+    eapply RB; now symmetry.
+Qed.
+
+
+Lemma mkPair_isLRPair {Γ A A' A1 B B' B1 a1 b1 l}
+  (RΣ0 : [Γ ||-<l> tSig A B ≅ tSig A' B'])
+  (RΣ := normRedΣ RΣ0)
+  (RA1 : [Γ ||-<l> A ≅ A1])
+  (RB1 : [Γ ||-<l> B[a1..] ≅ B1[a1..]])
+  (Ra1 : [Γ ||-<l> a1 : _ | RA1])
+  (Rb1 : [Γ ||-<l> b1 : _ | RB1])
+: isLRPair RΣ (tPair A1 B1 a1 b1).
+Proof.
+  escape.
+  unshelve eapply PairLRPair; tea; intros.
+  - now unshelve now eapply irrLR, wkLR.
+  - now unshelve now eapply irrLREq, wkLR; tea; rewrite subst_ren_subst_mixed.
+Qed.
+
+Definition pairSigRedTm {Γ A A' A1 B B' B1 a1 b1 l}
+  (RΣ0 : [Γ ||-<l> tSig A B ≅ tSig A' B'])
+  (RΣ1 : [Γ ||-<l> tSig A B ≅ tSig A1 B1])
+  (RΣ := normRedΣ RΣ0)
+  (Ra1 : [Γ ||-<l> a1 : _ | redΣdom RΣ0])
+  (Rb1 : [Γ ||-<l> b1 : _ | redΣcodfst RΣ0 Ra1])
+: SigRedTm RΣ (tPair A1 B1 a1 b1).
+Proof.
+  exists (tPair A1 B1 a1 b1); pose proof (RA := redΣdom RΣ1);
+    pose proof (RB := redΣcodfst RΣ1 (fst (irrLR _ RA _ _) Ra1)).
+  + eapply redtmwf_refl; cbn.
+    assert (wfΓ : [|- Γ]) by (escape ; gtyping).
+    assert [_ ||-<l> a1 : _ | urefl RA ] by now eapply irrLRConv.
+    pose proof (instKripkeFamConv wfΓ (normRedΣ RΣ1).(PolyRed.posRed)).
+    assert [_ ||-<l> b1 : _ | urefl RB ] by now eapply irrLRConv.
+    escape.
+    eapply ty_conv; [ eapply ty_pair; tea| now symmetry].
+  + now unshelve now eapply mkPair_isLRPair; eapply irrLR.
+Defined.
+
+Lemma pairCongRed {Γ A A' B B' a a' b b' l}
+  (RΣ0 : [Γ ||-<l> tSig A B ≅ tSig A' B'])
+  (RΣ := normRedΣ RΣ0)
+  (RΣ' := LRSig' RΣ)
+  (RA : [Γ ||-<l> A ≅ A'])
+  (RBa : [Γ ||-<l> B[a..] ≅ B'[a'..] ])
+  (Ra : [Γ ||-<l> a ≅ a' : A | RA])
+  (Rb : [Γ ||-<l> b ≅ b' : _ | RBa ]) :
+  [Γ ||-<l> tPair A B a b ≅ tPair A' B' a' b' : _ | RΣ'].
+Proof.
+  assert (wfΓ : [|-Γ]) by (escape; gtyping).
+  pose proof (convtyB := redΣcod RΣ').
+  pose proof (wtB' := escape (symmetry (instKripkeFamConv wfΓ RΣ.(PolyRed.posRed)))).
+  unshelve epose proof (pairFstRed' RA convtyB wtB' RBa Ra Rb) as (ff'&fa&fa').
+  pose proof (RBconv := instKripkeSubst (kripkeLRlrefl RΣ.(PolyRed.posRed)) RA (fst (irrLR _ _ _ _) fa)).
+
+  unshelve eapply build_sigRedTmEq'.
+  + unshelve eapply pairSigRedTm; eapply lrefl; tea; now eapply irrLR.
+  + unshelve eapply pairSigRedTm; tea; eapply urefl. now eapply irrLR.
+    eapply irrLRConv; tea; eapply (instKripkeSubst (kripkeLRlrefl RΣ.(PolyRed.posRed)) RA Ra).
+  + cbn; eapply irrLR, pairFstRed; tea.
+  + unshelve now cbn; eapply irrLR; eapply pairSndRed; tea; symmetry.
+    now eapply (instKripkeSubst RΣ.(PolyRed.posRed)).
+Qed.
+
+End SigmaRed.
+
+
+
+
+
