theories/Validity/Introductions/Nat.v
@@ -1,6 +1,6 @@
 From LogRel Require Import Utils Syntax.All GenericTyping LogicalRelation.
 From LogRel.LogicalRelation Require Import Properties.
-From LogRel.LogicalRelation.Introductions Require Import Universe SimpleArr Application.
+From LogRel.LogicalRelation.Introductions Require Import Universe SimpleArr Application Nat.
 From LogRel.Validity Require Import Validity Irrelevance Properties Universe Pi SimpleArr Var Application.
 
 Set Universe Polymorphism.
@@ -11,44 +11,15 @@ Context `{GenericTypingProperties}.
 
 Set Printing Primitive Projection Parameters.
 
-Lemma natRedTy {Γ} : [|- Γ] -> [Γ ||-Nat tNat ≅ tNat].
-Proof.
-  constructor; eapply redtywf_refl; gen_typing.
-Qed.
-
-Definition natRed {Γ l} (wfΓ : [|- Γ]) : [Γ ||-<l> tNat] :=
-  LRNat_ l (natRedTy wfΓ).
-
 Lemma natValid {Γ Γ' l} (VΓ : [||-v Γ ≅ Γ']) : [Γ ||-v<l> tNat | VΓ].
 Proof.
   unshelve econstructor; intros; now eapply natRed.
 Defined.
 
-Lemma natURedTm {Δ} (wfΔ : [|-Δ]) : URedTm zero Δ tNat.
-Proof.
-  exists tNat; [| constructor].
-  eapply redtmwf_refl; gen_typing.
-Defined.
-
-Lemma natTermRed {Δ} (wfΔ : [|-Δ]) : [Δ ||-<one> tNat : U | LRU_ (redUOneCtx wfΔ)].
-Proof.
-  unshelve econstructor; try now eapply natURedTm.
-  1: cbn; gtyping.
-  eapply redTyRecBwd; now eapply natRed.
-Defined.
-
-Lemma natTermValid {Γ} (VΓ : [||-v Γ]):  [Γ ||-v<one> tNat : U | VΓ | UValid VΓ].
+Lemma natValidU {Γ} (VΓ : [||-v Γ]):  [Γ ||-v<one> tNat : U | VΓ | UValid VΓ].
 Proof.
   constructor; intros; eapply natTermRed.
 Qed.
-
-Lemma zeroRed {Γ l A B} {NN : [Γ ||-Nat A ≅ B]} : [Γ ||-<l> tZero : _ | LRNat_ l NN].
-Proof.
-  assert [|-Γ] by (pose (LRNat_ l NN); escape; gtyping).
-  exists tZero tZero.
-  1-3: gtyping.
-  constructor.
-Defined.
 
 Lemma zeroValid {Γ Γ' l} (VΓ : [||-v Γ ≅ Γ']):
   [Γ ||-v<l> tZero : tNat | VΓ | natValid VΓ].
@@ -56,36 +27,6 @@ Proof.
   constructor; intros; cbn; unshelve eapply zeroRed; tea.
   3: now eapply natRedTy.
 Qed.
-
-Lemma succRed {Γ l A A' n n'} {NN : [Γ ||-Nat A ≅ A']} :
-  [Γ ||-<l> n ≅ n' : _ | LRNat_ l NN] ->
-  [Γ ||-<l> tSucc n ≅ tSucc n' : _ | LRNat_ l NN].
-Proof.
-  intros h; pose proof (h' :=h); inversion h'; subst.
-  escape; exists (tSucc n) (tSucc n').
-  1,2: eapply redtmwf_refl; eapply ty_succ; gen_typing.
-  + eapply convtm_succ; eapply convtm_exp; gen_typing.
-  + now constructor.
-Defined.
-
-(* Lemma succRed {Γ A A' l n} {NN : [Γ ||-Nat A ≅ A']} :
-  [Γ ||-<l> n : _ | LRNat_ l NN] ->
-  [Γ ||-<l> tSucc n : _ | LRNat_ l NN].
-Proof. eapply succRedEq. Defined. *)
-
-
-(* Lemma succRedInv {Γ l n m } {NN : [Γ ||-Nat tNat]} :
-  [Γ ||-<l> tSucc n ≅ tSucc m : _ | LRNat_ l NN] ->
-  [Γ ||-<l> n ≅ m : _ | LRNat_ l NN].
-Proof.
-  intros RSn; inversion RSn; subst.
-  unshelve epose proof (redtmwf_whnf redL _); try constructor.
-  unshelve epose proof (redtmwf_whnf redR _); try constructor.
-  subst. inversion prop; subst; tea.
-  match goal with H : [ _ ||-NeNf _ ≅ _ : _] |- _ => destruct H as [?? refl] end.
-  apply convneu_whne in refl; inv_whne.
-Qed. *)
-
 
 Lemma succValid' {Γ Γ' A A' l n n'} (VΓ : [||-v Γ ≅ Γ'])
   (VN : [Γ ||-v<l> A ≅ A' | VΓ])
@@ -106,90 +47,6 @@ Proof.
   constructor; intros; cbn; instValid Vσσ'.
   unshelve eapply succRed; cycle 3; first [eapply natRedTy| tea].
 Qed.
-
-Lemma elimSuccHypTy_subst {P} σ :
-  elimSuccHypTy P[up_term_term σ] = (elimSuccHypTy P)[σ].
-Proof.
-  unfold elimSuccHypTy.
-  cbn. rewrite shift_up_eq.
-  erewrite liftSubstComm.
-  rewrite up_liftSubst_eq.
-  now rewrite wk1_ren.
-  Unshelve. all: tea; constructor.
-Qed.
-
-Lemma liftSubst_singleSubst_eq {t u v: term} : t[u]⇑[v..] = t[u[v..]..].
-Proof. now bsimpl. Qed.
-
-Section NatElimRedEq.
-  Context {Γ l P Q hs hs' hz hz'}
-    (* (wfΓ : [|- Γ]) *)
-    (NN : [Γ ||-Nat tNat ≅ tNat])
-    (RN := LRNat_ _ NN)
-    (* (RP : [Γ,, tNat ||-<l> P])
-    (RQ : [Γ,, tNat ||-<l> Q]) *)
-    (WtP : [Γ ,, tNat |- P])
-    (WtQ : [Γ ,, tNat |- Q])
-    (eqPQ : [Γ,, tNat |- P ≅ Q])
-    (RPQext : forall n n' (Rn : [Γ ||-<l> n ≅ n' : _ | RN]),
-      [Γ ||-<l> P[n..] ≅ Q[n'..]])
-    (RPQz := RPQext _ _ zeroRed)
-    (Rhz : [Γ ||-<l> hz ≅ hz' : _ | RPQz])
-    (RPQs : [Γ ||-<l> elimSuccHypTy P ≅ elimSuccHypTy Q])
-    (Rhs : [Γ ||-<l> hs ≅ hs' : _ | RPQs ]) .
-
-  #[local]
-  Lemma RPext : forall n n' (Rn : [Γ ||-<l> n ≅ n' : _ | RN]),
-      [Γ ||-<l> P[n..] ≅ P[n'..]].
-  Proof.
-    intros; etransitivity; [|symmetry];  eapply RPQext; tea; now eapply urefl.
-  Qed.
-
-  Lemma natElimRedEqAux :
-    (forall n n' (Rnn' : [Γ ||-<l> n ≅ n' : _ | RN]),
-      [Γ ||-<l> tNatElim P hz hs n ≅ tNatElim Q hz' hs' n' : _ | RPQext _ _ Rnn' ]) ×
-    (forall n n' (Rnn' : NatPropEq Γ n n') (RP : [Γ ||-<l> P[n..] ≅ Q[n'..]]),
-      [Γ ||-<l> tNatElim P hz hs n ≅ tNatElim Q hz' hs' n' : _ | RP ]).
-  Proof.
-    apply NatRedEqInduction.
-    - intros t u  nfL nfR redL redR ? prop ih.
-      set (Rtu := Build_NatRedTmEq _ _ _ _ _ _ : [Γ ||-<l> t ≅ u : _ | RN]).
-      pose proof (redTmFwd' Rtu) as []; eapply redSubstTmEq.
-      + unshelve eapply irrLRConv, ih;
-        first [eapply RPQext| eapply RPext]; tea; now symmetry.
-      + escape; eapply redtm_natelim; tea; gen_typing.
-      + escape; eapply redtm_natelim; tea; [..| gtyping].
-        1,2: now eapply ty_conv.
-    - intros; eapply redSubstTmEq.
-      + eapply irrLR, Rhz.
-      + escape; eapply redtm_natElimZero; tea.
-      + escape; eapply redtm_natElimZero; tea.
-        1,2: now eapply ty_conv.
-    - intros n n' Rn ih ?; change [Γ ||-<l> n ≅ n' : _ | RN] in Rn.
-      eapply redSubstTmEq; cycle 1.
-      + escape; eapply redtm_natElimSucc; tea.
-      + escape; eapply redtm_natElimSucc; tea.
-        1,2: now eapply ty_conv.
-      + assert [Γ ||-<l> arr P[n..] P[(tSucc n)..] ≅ arr Q[n'..] Q[(tSucc n')..]].
-        1: now eapply ArrRedTy; eapply RPQext;[|eapply succRed].
-        unshelve eapply simple_appcongTerm; [..| eauto]; tea.
-        unshelve (eapply irrLREq, appcongTerm; tea; now rewrite subst_arr, liftSubst_singleSubst_eq).
-        now rewrite 2!subst_arr, 2!liftSubst_singleSubst_eq.
-    - intros n n' Rn RP0.
-      pose proof (neNfTermEq RN Rn).
-      eapply reflectLR.
-      + escape; now eapply ty_natElim.
-      + eapply ty_conv ; [| eapply escapeEq; now symmetry].
-        escape; eapply ty_natElim; tea.
-        all: now eapply ty_conv.
-      + escape ; destruct Rn; now eapply convneu_natElim.
-  Qed.
-
-  Lemma natElimRedEq :
-    (forall n n' (Rnn' : [Γ ||-<l> n ≅ n' : _ | RN]),
-      [Γ ||-<l> tNatElim P hz hs n ≅ tNatElim Q hz' hs' n' : _ | RPQext _ _ Rnn' ]).
-  Proof. intros; now apply (fst natElimRedEqAux). Qed.
-End NatElimRedEq.
 
 
 Section NatElimValid.
@@ -255,9 +112,7 @@ Section NatElimRedValid.
     (VN := natValid (l:=l) VΓ)
     (VΓN := validSnoc VΓ VN)
     { P P' hz hz' hs hs'}
-    (* (VP : [Γ ,, tNat ||-v<l> P | VΓN]) *)
     (VP : [Γ ,, tNat ||-v<l> P ≅ P' | VΓN ])
-    (* (VP' := ureflValidTy VPP') *)
     (VPz := substS VP (zeroValid VΓ))
     (Vhz : [Γ ||-v<l> hz ≅ hz' : P[tZero..] | VΓ | VPz])
     (Vhs : [Γ ||-v<l> hs ≅ hs' : _ | VΓ | elimSuccHypTyValid VΓ VP]).
